fstar/MLS.TreeSync.fst
@@ -1,9 +1,14 @@
 module MLS.TreeSync
 
-open Comparse.Bytes
+open Comparse
+open MLS.Crypto
+open MLS.NetworkTypes
+open MLS.NetworkBinder
 open MLS.Utils
 open MLS.Tree
 open MLS.TreeSync.Types
+open MLS.TreeSync.ParentHash
+open MLS.Result
 
 #set-options "--fuel 1 --ifuel 1"
 
@@ -50,15 +55,121 @@ val tree_remove: #bytes:Type0 -> {|bytes_like bytes|} -> #l:nat -> #i:tree_index
 let tree_remove #bytes #bl #l #i t li =
   tree_blank_path t li None
 
-val apply_path: #bytes:Type0 -> {|bytes_like bytes|} -> #l:nat -> #i:tree_index l -> #li:leaf_index l i -> treesync bytes l i -> pathsync bytes l i li -> treesync bytes l i
-let rec apply_path #bytes #bl #l #i #li t p =
-  match t,p with
-  | TLeaf _, PLeaf m' -> TLeaf m'
-  | TNode _ left right, PNode onp next ->
-     if is_left_leaf li
-     then TNode onp (apply_path left next) right
-     else TNode onp left (apply_path right next)
+val compute_new_np_and_ph: #bytes:Type0 -> {|crypto_bytes bytes|} -> #l:nat -> #i:tree_index l -> option (external_content bytes) -> treesync bytes l i -> mls_bytes bytes -> result (option (node_package_t bytes) & mls_bytes bytes)
+let compute_new_np_and_ph #bytes #cb #l #i opt_ext_content sibling parent_parent_hash =
+  let new_opt_content =
+    match opt_ext_content with
+    | Some ext_content -> Some ({
+      version = 0;
+      unmerged_leaves = [];
+      parent_hash = parent_parent_hash;
+      content = ext_content;
+    } <: node_package_t bytes)
+    | None -> None
+  in
+  new_parent_parent_hash <-- (
+    match opt_ext_content with
+    | Some ext_content ->
+      compute_parent_hash ext_content.content parent_parent_hash sibling
+    | None -> return parent_parent_hash
+  );
+  return (new_opt_content, new_parent_parent_hash)
 
+val compute_leaf_parent_hash_from_external_path: #bytes:Type0 -> {|crypto_bytes bytes|} -> #l:nat -> #i:tree_index l -> #li:leaf_index l i -> t:treesync bytes l i -> external_pathsync bytes l i li -> mls_bytes bytes -> result (mls_bytes bytes)
+let rec compute_leaf_parent_hash_from_external_path #bytes #cb #l #i #li t p parent_parent_hash =
+  match t, p with
+  | TLeaf old_lp, PLeaf new_lp -> (
+    return parent_parent_hash
+  )
+  | TNode _ left right, PNode opt_ext_content p_next ->
+    let (child, sibling) = get_child_sibling t li in
+    tmp <-- compute_new_np_and_ph opt_ext_content sibling parent_parent_hash;
+    let (_,  new_parent_parent_hash) = tmp in
+    if is_left_leaf li then
+      compute_leaf_parent_hash_from_external_path left p_next new_parent_parent_hash
+    else
+      compute_leaf_parent_hash_from_external_path right p_next new_parent_parent_hash
+
+val get_external_path_leaf: #bytes:Type0 -> {|crypto_bytes bytes|} -> #l:nat -> #i:tree_index l -> #li:leaf_index l i -> external_pathsync bytes l i li -> leaf_package_t bytes
+let rec get_external_path_leaf #bytes #cb #l #i #li p =
+  match p with
+  | PLeaf lp -> lp
+  | PNode _ p_next -> get_external_path_leaf p_next
+
+val set_external_path_leaf: #bytes:Type0 -> {|crypto_bytes bytes|} -> #l:nat -> #i:tree_index l -> #li:leaf_index l i -> external_pathsync bytes l i li -> leaf_package_t bytes -> external_pathsync bytes l i li
+let rec set_external_path_leaf #bytes #cb #l #i #li p lp =
+  match p with
+  | PLeaf _ -> PLeaf lp
+  | PNode p_content p_next -> PNode p_content (set_external_path_leaf p_next lp)
+
+val get_leaf_package_tbs: #bytes:Type0 -> {|bytes_like bytes|} -> leaf_package_t bytes -> bytes -> result bytes
+let get_leaf_package_tbs #bytes #bl lp group_id =
+    ln <-- leaf_package_to_network lp;
+    if not (length group_id < pow2 30) then
+      internal_failure "sign_leaf: group_id is too long"
+    else (
+      let ln_tbs = ({
+        data = ln.data;
+        group_id = (match ln.data.source with |LNS_update () |LNS_commit() -> group_id |_ -> ());
+      } <: leaf_node_tbs_nt bytes) in
+      return (serialize (leaf_node_tbs_nt bytes) ln_tbs)
+    )
+
+val external_path_is_valid: #bytes:Type0 -> {|crypto_bytes bytes|} -> #l:nat -> #i:tree_index l -> #li:leaf_index l i -> t:treesync bytes l i -> external_pathsync bytes l i li -> bytes -> result bool
+let external_path_is_valid #bytes #cb #l #i #li t p group_id =
+  let old_lp = leaf_at t li in
+  let new_lp = get_external_path_leaf p in
+  //TODO: something stating that new_lp is related to old_lp
+  computed_parent_hash <-- compute_leaf_parent_hash_from_external_path t p root_parent_hash;
+  tbs <-- get_leaf_package_tbs new_lp group_id;
+  verification_key <-- (
+    if not (length new_lp.credential.signature_key = sign_public_key_length #bytes) then
+      error "external_path_is_valid: verification key has wrong length"
+    else
+      return (new_lp.credential.signature_key <: sign_public_key bytes)
+  );
+  signature <-- (
+    if not (length new_lp.signature = sign_signature_length #bytes) then
+      error "external_path_is_valid: signature has wrong length"
+    else
+      return (new_lp.signature <: sign_signature bytes)
+  );
+  signature_ok <-- verify_with_label verification_key (string_to_bytes #bytes "LeafNodeTBS") tbs signature;
+  let parent_hash_ok = (new_lp.source = LNS_commit () && (new_lp.parent_hash <: bytes) = computed_parent_hash) in
+  return (signature_ok && parent_hash_ok)
+
+val external_path_to_valid_external_path: #bytes:Type0 -> {|crypto_bytes bytes|} -> #l:nat -> #i:tree_index l -> #li:leaf_index l i -> t:treesync bytes l i -> external_pathsync bytes l i li -> bytes -> sign_private_key bytes -> sign_nonce bytes -> result (external_pathsync bytes l i li)
+let external_path_to_valid_external_path #bytes #cb #l #i #li t p group_id sign_key nonce =
+  computed_parent_hash <-- compute_leaf_parent_hash_from_external_path t p root_parent_hash;
+  let lp = get_external_path_leaf p in
+  if not (lp.source = LNS_commit ()) then
+    error "external_path_to_valid_external_path: source is not a commit"
+  else (
+    let new_lp = { lp with parent_hash = computed_parent_hash; } in
+    new_lp_tbs <-- get_leaf_package_tbs new_lp group_id;
+    new_signature <-- sign_with_label sign_key (string_to_bytes #bytes "LeafNodeTBS") new_lp_tbs nonce;
+    return (set_external_path_leaf p ({ new_lp with signature = new_signature }))
+  )
+
+val apply_external_path_aux: #bytes:Type0 -> {|crypto_bytes bytes|} -> #l:nat -> #i:tree_index l -> #li:leaf_index l i -> t:treesync bytes l i -> external_pathsync bytes l i li -> mls_bytes bytes -> result (treesync bytes l i)
+let rec apply_external_path_aux #bytes #cb #l #i #li t p parent_parent_hash =
+  match t, p with
+  | TLeaf _, PLeaf lp -> return (TLeaf (Some lp))
+  | TNode _ left right, PNode opt_ext_content p_next ->
+    let (child, sibling) = get_child_sibling t li in
+    tmp <-- compute_new_np_and_ph opt_ext_content sibling parent_parent_hash;
+    let (new_opt_content, new_parent_parent_hash) = tmp in
+    if is_left_leaf li then (
+      new_left <-- (apply_external_path_aux left p_next new_parent_parent_hash);
+      return (TNode new_opt_content new_left right)
+    ) else (
+      new_right <-- (apply_external_path_aux right p_next new_parent_parent_hash);
+      return (TNode new_opt_content left new_right)
+    )
+
+val apply_external_path: #bytes:Type0 -> {|crypto_bytes bytes|} -> #l:nat -> #i:tree_index l -> #li:leaf_index l i -> t:treesync bytes l i -> external_pathsync bytes l i li -> result (treesync bytes l i)
+let apply_external_path #bytes #cb #l #i #li t p =
+  apply_external_path_aux t p root_parent_hash
 
 (*** Tree extension / truncation ***)
 
